StackSubtyping.dfy
@@ -1,35 +1,35 @@
 
 include "StackSyntax.dfy"
 
-predicate method Prefix<A(==)>(s: seq<A>, t: seq<A>) {
-  |s| <= |t| &&
-    forall i | 0 <= i < |s| :: s[i] == t[i]
+predicate method Prefix<A(==)>(s: List<A>, t: List<A>) {
+  Length(s) <= Length(t) &&
+    forall i | 0 <= i < Length(s) :: Nth(i, s) == Nth(i, t)
 }
 
-lemma PrefixReflexive<A(==)>(s: seq<A>)
+lemma PrefixReflexive<A(==)>(s: List<A>)
   ensures Prefix(s, s)
 {
 }
 
-lemma PrefixAntisymmetric<A(==)>(s: seq<A>, t: seq<A>)
+lemma PrefixAntisymmetric<A(==)>(s: List<A>, t: List<A>)
   requires Prefix(s, t)
   requires Prefix(t, s)
   ensures s == t
 {
 }
 
-lemma PrefixTransitive<A(==)>(r: seq<A>, s: seq<A>, t: seq<A>)
+lemma PrefixTransitive<A(==)>(r: List<A>, s: List<A>, t: List<A>)
   requires Prefix(r, s)
   requires Prefix(s, t)
   ensures  Prefix(r, t)
 {
 }
 
-lemma PrefixSplit<A(==)>(n: nat, xs: seq<A>, ys: seq<A>)
-  requires n < |xs|
+lemma PrefixSplit<A(==)>(n: nat, xs: List<A>, ys: List<A>)
+  requires n < Length(xs)
   requires Prefix(xs, ys)
-  ensures  Prefix(xs[..n], ys[..n])
-  ensures  Prefix(xs[n..], ys[n..])
+  ensures  Prefix(Drop(n, xs), Drop(n, ys))
+  ensures  Prefix(Take(n, xs), Take(n, ys))
 {
 }
 
@@ -37,12 +37,12 @@ predicate method SubPhiSigned(p: bool, s: Phi, t: Phi)
   decreases s, t
 {
   var s, t := s.out, t.out;
-  (if p then |s| <= |t|
-        else |t| <= |s|) &&
-  forall i | 0 <= i < |if p then s else t| ::
-    SubPhiSigned(!p, s[i].0, t[i].0) &&
-    if p then Prefix(s[i].1, t[i].1)
-         else Prefix(t[i].1, s[i].1)
+  (if p then Length(s) <= Length(t)
+        else Length(t) <= Length(s)) &&
+  forall i | 0 <= i < Length(if p then s else t) ::
+    SubPhiSigned(!p, Nth(i, s).0, Nth(i, t).0) &&
+    if p then Prefix(Nth(i, s).1, Nth(i, t).1)
+         else Prefix(Nth(i, t).1, Nth(i, s).1)
 }
 
 predicate method SubPhi(s: Phi, t: Phi)
@@ -68,11 +68,11 @@ lemma SubPhiAntisymmetricSigned(p: bool, s: Phi, t: Phi)
   ensures  s == t
 {
   var (s, t) := (s.out, t.out);
-  forall i | 0 <= i < |s|
-    ensures s[i] == t[i]
+  forall i | 0 <= i < Length(s)
+    ensures Nth(i, s) == Nth(i, t)
   {
-    PrefixAntisymmetric(s[i].1, t[i].1);
-    SubPhiAntisymmetricSigned(p, s[i].0, t[i].0);
+    PrefixAntisymmetric(Nth(i, s).1, Nth(i, t).1);
+    SubPhiAntisymmetricSigned(p, Nth(i, s).0, Nth(i, t).0);
   }
   assert s == t;
 }
@@ -93,15 +93,15 @@ lemma SubPhiTransitiveSigned(p: bool, r: Phi, s: Phi, t: Phi)
   ensures  SubPhiSigned(p, r, t)
 {
   var (r, s, t) := (r.out, s.out, t.out);
-  forall i | 0 <= i < |if p then r else t|
-    ensures SubPhiSigned(!p, r[i].0, t[i].0);
+  forall i | 0 <= i < Length(if p then r else t)
+    ensures SubPhiSigned(!p, Nth(i, r).0, Nth(i, t).0);
   {
     if p {
-      PrefixTransitive(r[i].1, s[i].1, t[i].1);
+      PrefixTransitive(Nth(i, r).1, Nth(i, s).1, Nth(i, t).1);
     } else {
-      PrefixTransitive(t[i].1, s[i].1, r[i].1);
+      PrefixTransitive(Nth(i, t).1, Nth(i, s).1, Nth(i, r).1);
     }
-    SubPhiTransitiveSigned(!p, r[i].0, s[i].0, t[i].0);
+    SubPhiTransitiveSigned(!p, Nth(i, r).0, Nth(i, s).0, Nth(i, t).0);
   }
 }
 
@@ -117,24 +117,24 @@ lemma SubPhiTransitive(r: Phi, s: Phi, t: Phi)
 lemma SubPhiAllContravariantSigned(p: bool, s: Phi, t: Phi)
   decreases s, t
   requires SubPhiSigned(p, s, t)
-  ensures  forall i | 0 <= i < |if p then s.out else t.out| ::
-             SubPhiSigned(!p, s.out[i].0, t.out[i].0)
+  ensures  forall i | 0 <= i < Length(if p then s.out else t.out) ::
+             SubPhiSigned(!p, Nth(i, s.out).0, Nth(i, t.out).0)
 {
   var (s, t) := (s.out, t.out);
-  forall i | 0 <= i < |if p then s else t|
-    ensures SubPhiSigned(!p, s[i].0, t[i].0)
+  forall i | 0 <= i < Length(if p then s else t)
+    ensures SubPhiSigned(!p, Nth(i, s).0, Nth(i, t).0)
   {
-    SubPhiAllContravariantSigned(!p, s[i].0, t[i].0);
+    SubPhiAllContravariantSigned(!p, Nth(i, s).0, Nth(i, t).0);
   }
 }
 
 lemma SubPhiAllContravariant(s: Phi, t: Phi)
   requires SubPhi(s, t)
-  ensures  forall i | 0 <= i < |s.out| :: SubPhi(t.out[i].0, s.out[i].0)
+  ensures  forall i | 0 <= i < Length(s.out) :: SubPhi(Nth(i, t.out).0, Nth(i, s.out).0)
 {
   SubPhiAllContravariantSigned(true, s, t);
-  forall i | 0 <= i < |s.out| {
-    SubPhiFlip(t.out[i].0, s.out[i].0);
+  forall i | 0 <= i < Length(s.out) {
+    SubPhiFlip(Nth(i, t.out).0, Nth(i, s.out).0);
   }
 }
 
@@ -144,10 +144,10 @@ lemma SubPhiFlipSigned(p: bool, s: Phi, t: Phi)
   ensures  SubPhiSigned(!p, t, s)
 {
   var (s, t) := (s.out, t.out);
-  forall i | 0 <= i < |if p then s else t|
-    ensures SubPhiSigned(p, t[i].0, s[i].0)
+  forall i | 0 <= i < Length(if p then s else t)
+    ensures SubPhiSigned(p, Nth(i, t).0, Nth(i, s).0)
   {
-    SubPhiFlipSigned(!p, s[i].0, t[i].0);
+    SubPhiFlipSigned(!p, Nth(i, s).0, Nth(i, t).0);
   }
 }
 
@@ -163,17 +163,17 @@ lemma SubPhiFlip(s: Phi, t: Phi)
 }
 
 lemma SubPhiSplit(n: nat, Phi1: Phi, Phi2: Phi)
-  requires n < |Phi1.out|
+  requires n < Length(Phi1.out)
   requires SubPhi(Phi1, Phi2)
-  ensures  SubPhi(MkPhi(Phi1.out[..n]), MkPhi(Phi2.out[..n]))
-  ensures  SubPhi(MkPhi(Phi1.out[n..]), MkPhi(Phi2.out[n..]))
+  ensures  SubPhi(MkPhi(Take(n, Phi1.out)), MkPhi(Take(n, Phi2.out)))
+  ensures  SubPhi(MkPhi(Drop(n, Phi1.out)), MkPhi(Drop(n, Phi2.out)))
 {
 }
 
 lemma SubPhiJoin(Phi1a: Phi, Phi1b: Phi, Phi2a: Phi, Phi2b: Phi)
   requires SubPhi(Phi1a, Phi2a)
   requires SubPhi(Phi1b, Phi2b)
-  requires |Phi1a.out| == |Phi2a.out|
-  ensures  SubPhi(MkPhi(Phi1a.out + Phi1b.out), MkPhi(Phi2a.out + Phi2b.out))
+  requires Length(Phi1a.out) == Length(Phi2a.out)
+  ensures  SubPhi(MkPhi(Append(Phi1a.out, Phi1b.out)), MkPhi(Append(Phi2a.out, Phi2b.out)))
 {
 }
